Mica/FOL/Printing.lean
@@ -68,6 +68,7 @@ def BinOp.toSMTLIB : BinOp τ₁ τ₂ τ₃ → String
   | .ge    => ">="
   | .eq    => "="
   | .seqConcat => "seq.++"
+  | .seqNth => "seq.nth"
   | .seqPrefixOf => "seq.prefixof"
   | .seqSuffixOf => "seq.suffixof"
   | .fpAdd => "fp.add roundNearestTiesToEven"
@@ -81,6 +82,7 @@ def BinOp.toSMTLIB : BinOp τ₁ τ₂ τ₃ → String
   | .uninterpreted name _ _ _ => name
 
 def TerOp.toSMTLIB : TerOp τ₁ τ₂ τ₃ τ₄ → String
+  | .seqExtract => "seq.extract"
   | .uninterpreted name _ _ _ _ => name
 
 def UnPred.toSMTLIB : UnPred τ → String
@@ -254,6 +256,7 @@ private def termStr (p : Prec) : {τ : Srt} → Term τ → String
     | .ge    => parens (Prec.lt .cmp p) s!"{termStr .add a} >= {termStr .add b}"
     | .eq    => parens (Prec.lt .cmp p) s!"{termStr .add a} = {termStr .add b}"
     | .seqConcat => parens (Prec.lt .add p) s!"{termStr .add a} ++ {termStr .mul b}"
+    | .seqNth => s!"nth({termStr .bottom a}, {termStr .bottom b})"
     | .seqPrefixOf => s!"prefixOf({termStr .bottom a}, {termStr .bottom b})"
     | .seqSuffixOf => s!"suffixOf({termStr .bottom a}, {termStr .bottom b})"
     | .fpAdd => parens (Prec.lt .add p) s!"{termStr .add a} +. {termStr .mul b}"
@@ -266,6 +269,7 @@ private def termStr (p : Prec) : {τ : Srt} → Term τ → String
     | .vcons => parens (Prec.lt .top p) s!"{termStr .top a} :: {termStr .top b}"
     | .uninterpreted name _ _ _ => s!"{name}({termStr .bottom a}, {termStr .bottom b})"
   | _, .terop op a b c => match op with
+    | .seqExtract => s!"extract({termStr .bottom a}, {termStr .bottom b}, {termStr .bottom c})"
     | .uninterpreted name _ _ _ _ =>
       s!"{name}({termStr .bottom a}, {termStr .bottom b}, {termStr .bottom c})"
   | _, .ite c t e  => parens (Prec.lt .bottom p) s!"if {termStr .bottom c} then {termStr .bottom t} else {termStr .bottom e}"
